Bdd/Restrict.lean
@@ -1,0 +1,50 @@
+import Bdd.Basic
+import Bdd.Nary
+
+namespace Restrict
+
+structure State (n) (m) where
+  visited : Vector (Option (Pointer m)) m
+  newheap : Vector (Node n m) m
+
+def lookup (j : Fin m) : StateM (State n m) (Option (Pointer m)) := fun ⟨V, M⟩ ↦ ⟨V[j], V, M⟩
+def store (j : Fin m) (p : Pointer m) : StateM (State n m) (Pointer m) := fun ⟨V, M⟩ ↦ ⟨p, V.set j p, M⟩
+def setj (j : Fin m) : Node n m → StateM (State n m) Unit := fun N ⟨V, M⟩ ↦ ⟨(), V, M.set j N⟩
+
+def restrict_helper (O : OBdd n m) (b : Bool) (i : Fin n) :
+    StateM (State n m) (Pointer m) := do
+  let r := O.1.root
+  match hr : r with
+  | .terminal _ => return r
+  | .node j =>
+    -- TODO: there must be a nicer way to write this get-match-return-or-else dance.
+    let cached ← lookup j
+    match cached with
+    | some p => return p
+    | none =>
+      let N := O.1.heap[j]
+      if N.var > i
+      then -- Orderedness guarantees that we won't encounter i anywhere in this subgraph, so keep it as is.
+        store j r
+      else
+        if N.var < i
+        then
+          let l ← restrict_helper (O.low  hr) b i
+          let h ← restrict_helper (O.high hr) b i
+          setj j ⟨N.var, l, h⟩
+          store j r
+        else -- Found a node with variable i, short-circuit to the appropriate child.
+          store j (if b then N.high else N.low)
+termination_by O
+
+def restrict (O : OBdd n m) (b : Bool) (i : Fin n) : Bdd n m :=
+  let ⟨r, _, M⟩ := restrict_helper O b i ⟨Vector.replicate m none, O.1.heap⟩
+  ⟨M,r⟩
+
+lemma restrict_ordered {O : OBdd n m} : Bdd.Ordered (restrict O b i) := sorry
+
+def orestrict (O : OBdd n m) (b : Bool) (i : Fin n) : OBdd n m := ⟨restrict O b i, restrict_ordered⟩
+
+lemma orestrict_evaluate {O : OBdd n m} : (orestrict O b i).evaluate = Nary.restrict (O.evaluate) b i := sorry
+
+end Restrict
